src/lib/communication/DY.Lib.Communication.Core.Lemmas.fst
@@ -374,6 +374,7 @@ let verify_message_proof #cinvs #a #ps tr sender receiver msg_bytes sk_receiver_
   )
 #pop-options
 
+#push-options "--ifuel 2 --fuel 1 --z3rlimit 20"
 val receive_authenticated_proof:
   {|invs:protocol_invariants|} ->
   #a:Type -> {| parseable_serializeable bytes a |} ->
@@ -410,11 +411,18 @@ let receive_authenticated_proof #invs #a tr higher_layer_preds comm_keys_ids rec
     let (Some vk_sender, tr) = get_public_key receiver comm_keys_ids.pki (LongTermSigKey comm_layer_sign_tag) sender tr in
     verify_message_proof #invs.crypto_invs #a tr sender receiver msg_signed_bytes None vk_sender;
     let (Some cm) = verify_message #a receiver msg_signed_bytes None vk_sender in
+    let Some msg_sign_t = parse com_message_t msg_signed_bytes in
+    let SigMessage msg_sign = msg_sign_t in
+    let Some sign_input = parse signature_input #parseable_serializeable_bytes_signature_input msg_sign.msg in
+    parse_serialize_inv_lemma #bytes a cm.payload;
+    serialize_wf_lemma a (is_publishable tr) cm.payload;
     let ((), tr) = trigger_event receiver (CommAuthReceiveMsg sender receiver (serialize a cm.payload)) tr in
     assert(tr_out == tr);
+    assert(Plain? sign_input);
     assert(trace_invariant tr_out);
     ()
   )
+#pop-options
 
 
 (**** Confidential and Authenticates Send and Receive Lemmas ****)
@@ -450,6 +458,7 @@ let encrypt_and_sign_message_proof #cinvs #a tr sender receiver payload pk_recei
   sign_message_proof #cinvs #com_send_byte tr sender receiver {b=enc_payload} (Some pk_receiver) sk_sender sign_nonce;
   ()
 
+#push-options "--ifuel 1 --z3rlimit 50"
 val send_confidential_authenticated_proof:
   {|invs:protocol_invariants|} ->
   #a:Type -> {| parseable_serializeable bytes a |} ->
@@ -496,11 +505,14 @@ let send_confidential_authenticated_proof #invs #a tr higher_layer_preds comm_ke
 
     encrypt_and_sign_message_proof tr' sender receiver payload pk_receiver sk_sender enc_nonce sign_nonce;
     let msg = encrypt_and_sign_message sender receiver payload pk_receiver sk_sender enc_nonce sign_nonce in
+    assert(trace_invariant tr');
+    assert(is_publishable tr' msg);
     let (msg_id, tr') = send_msg msg tr' in
     assert(tr_out == tr');
     assert(trace_invariant tr_out);
     ()
   )
+#pop-options
 
 
 #push-options "--ifuel 1 --z3rlimit 40"
@@ -563,6 +575,7 @@ let verify_and_decrypt_message_proof #cinvs #a tr sender receiver msg_encrypted_
   )
 #pop-options
 
+#push-options "--ifuel 1 --z3rlimit 25"
 val receive_confidential_authenticated_proof:
   {|invs:protocol_invariants|} ->
   #a:Type -> {| parseable_serializeable bytes a |} ->
@@ -604,9 +617,22 @@ let receive_confidential_authenticated_proof #invs #a tr higher_layer_preds comm
     let (Some vk_sender, tr) = get_public_key receiver comm_keys_ids.pki (LongTermSigKey comm_layer_sign_tag) sender tr in
     verify_and_decrypt_message_proof #invs.crypto_invs #a tr sender receiver msg_encrypted_signed sk_receiver vk_sender;
     let Some cm = verify_and_decrypt_message #a receiver sk_receiver vk_sender msg_encrypted_signed in
+    let Some cm_inner = verify_message #com_send_byte receiver msg_encrypted_signed (Some sk_receiver) vk_sender in
+    let Some msg_signed_t = parse com_message_t msg_encrypted_signed in
+    let SigMessage msg_signed = msg_signed_t in
+    let Some sign_input = parse signature_input msg_signed.msg in
+    let Encrypted _ _ _ pk_receiver = sign_input in
+    parse_serialize_inv_lemma #bytes a cm.payload;
+    assert(cm.sender == sender);
+    assert(is_well_formed a (is_knowable_by (principal_label receiver) tr) cm.payload);
+    assert(
+      event_triggered tr sender (CommConfAuthSendMsg sender receiver (serialize a cm.payload)) \/
+      is_corrupt tr (long_term_key_label sender)
+    );
     let ((), tr) = trigger_event receiver (CommConfAuthReceiveMsg sender receiver (serialize a cm.payload)) tr in
     assert(event_triggered tr receiver (CommConfAuthReceiveMsg sender receiver (serialize a cm.payload)));
     assert(trace_invariant tr);
     assert(tr == tr_out);
     ()
   )
+#pop-options
